[done] Mutant.v works now

theories/Generator.v
@@ -12,6 +12,7 @@ Fixpoint tlift (T : typ) (m : nat) :=
   end.
 
 (** ** Generate (Almost) SystemF *)
+(* collect all tvars  *)
 Definition gen_exact_tvar0' (E : env) : list (G typ) :=
   match count_tvar E with
   | O => []
@@ -21,6 +22,7 @@ Definition gen_exact_tvar0' (E : env) : list (G typ) :=
 Definition gen_exact_tvar0 (E : env) : (G (option typ)) :=
   oneOf_ (ret None) (map (fmap Some) (gen_exact_tvar0' E)).
 
+(* collect all vars *)
 Fixpoint gen_exact_var0' (E : env) : list typ :=
   match E with
   | empty => []
@@ -34,7 +36,7 @@ Definition gen_exact_from_var0' (E : env) : list (G typ) :=
 Definition gen_exact_from_var0 (E : env) : (G (option typ)) :=
   oneOf_ (ret None) (map (fmap Some) (gen_exact_from_var0' E)).
 
-(* There must be another way to write this *)
+(* collect all vars and tvars in [E] *)
 Definition gen_exact_typ0'  (E : env) : G typ :=
   let gs' := map (fun g => T <- g;; returnGen (arrow T T))
                 (gen_exact_tvar0' E) in
@@ -123,6 +125,86 @@ Fixpoint gen_ftvar0 (n : nat) (E : env) (acc : list typ) : list typ :=
 Definition gen_ftvar (E : env) : G (option typ) :=
   elems_ None (map Some (gen_ftvar0 0 E [])).
 
+
+(** Replace free/constant [typ's] in [t] with a new [typ] *)
+
+(** fetch_candidate_typs : 
+    list of free/constant [typ] in [T] under the context [E] 
+ *)
+Definition fetch_candidate_typs (T : typ) : list typ :=
+  let fix fetch_p T n :=
+    match T with
+    | top => true
+    | tvar n' => (** Check if it's free *)
+        n <=? n'
+    | arrow T1 T2 =>
+        ((fetch_p T1 n) && (fetch_p T2 n))%bool
+    | all T1 T2 =>
+        (** not precise here *)
+        ((fetch_p T1 n) && (fetch_p T2 (S n)))%bool
+    end in
+  let fix tunshift T n :=
+    match T with
+    | top => top
+    | tvar n' => tvar (n' - n)
+    | arrow T1 T2 => arrow (tunshift T1 n) (tunshift T2 n)
+    | all T1 T2 => all (tunshift T1 n) (tunshift T2 (S n))
+    end
+  in
+  let fix f T nbound :=
+    (if fetch_p T nbound then [tunshift T nbound] else [])
+      ++
+      (match T with
+       | arrow T1 T2 =>
+           (f T1 nbound) ++ (f T2 nbound)
+       | all T1 T2 =>
+           (f T1 nbound) ++ (f T2 (S nbound))
+       | _ => []
+       end) in
+  f T 0.  
+
+Definition gen_cand (T : typ) : G (option typ) :=
+  elems_ None (map Some (fetch_candidate_typs T)).
+
+(** 2 strategies here: 
+    - [replace_typ T T' n] :
+      replace part of type [T] equal to T'  with [tvar n]
+      (without considering sub)
+    - [mutate_typ E T] :
+      replace part of type [T] by consulting bound types in [E] 
+      (considerng sub typing)
+
+    Which one is better?
+ *)
+
+
+Fixpoint replace_typ T T' n : G typ :=
+  (** more likely to generate replacement *)
+  let g1 := (if T = T' ? then [(2 + n, ret (tvar n))] else [(1, ret T)])  in
+  let g2 :=
+    match T with
+    | arrow T1 T2 =>
+        T1' <- replace_typ T1 T' n ;;
+        T2' <- replace_typ T2 T' n ;;
+        ret (arrow T1' T2')
+    | all T1 T2 => 
+        T1' <- replace_typ T1 T' n ;;
+        T2' <- replace_typ T2 (tshift 0 T') (S n) ;;
+        ret (all T1' T2')
+    | _ => freq_ (ret T) g1
+    end in
+   freq_ (ret T) ((2 + n, g2) :: g1).
+
+Definition gen_replace T : G (option (typ * typ)) :=
+  oT1 <- gen_cand T ;;
+  match oT1 with
+  | Some T1 =>
+    T2 <- replace_typ (tshift 0 T) (tshift 0 T1) 0 ;;
+    (ret (Some (T1, T2)))
+  | None => ret None
+  end. 
+
+
 (** Generate terms from exact types *)
 Fixpoint gen_exact_term (n : nat) (E : env) (T : typ) : G (option term) :=
   match n with
@@ -150,8 +232,13 @@ Fixpoint gen_exact_term (n : nat) (E : env) (T : typ) : G (option term) :=
       let g3 :=
         T1 <- gen_exact_typ n E;; 
         t1 <- gen_exact_term n E (all T1 (tshift 0 T));;
-        returnGen (Some (tapp t1 T1))
-      in backtrack [(1, g0); (1, g1); (1, g2); (1, g3)]
+        returnGen (Some (tapp t1 T1)) in
+      let g4 :=
+        (** unrestricted: typ can be any *)
+        '(T2, T12) <- gen_replace T ;;
+        t1' <- gen_exact_term n E (all T2 T12) ;;
+        returnGen (Some (tapp t1' T2))
+      in backtrack [(1, g0); (1, g1); (1, g2); (1, g3); (1, g4)]
   end
 .      
 
@@ -165,128 +252,101 @@ Definition gen_exact (n : nat) : G (option term) :=
 (** ** Generate Subtype *)
 
 (** Find out super or sub type of the given [typ] in the environment *)
-Definition find_sub_tvar  
-           (E : env) (T2 : typ) : list typ :=
-  let n := count_tvar E in
-  let fix f n1 :=
-    match n1 with
-    | O => []
-    | S n1 => 
-        match get_bound E n1 with
-        | None => []
-        | Some T1 => 
-            let T' := match sub_check' E T1 T2 with
-                      | true => [T1]
-                      | _ => []
-                      end in
-            T' ++ (f n1)
-        end
-    end in
-  f n.
+(* Definition find_sub_tvar   *)
+(*            (E : env) (T2 : typ) : list typ := *)
+(*   let n := count_tvar E in *)
+(*   let fix f n1 := *)
+(*     match n1 with *)
+(*     | O => [] *)
+(*     | S n1 =>  *)
+(*         match get_bound E n1 with *)
+(*         | None => [] *)
+(*         | Some T1 =>  *)
+(*             let T' := match sub_check' E T1 T2 with *)
+(*                       | true => [T1] *)
+(*                       | _ => [] *)
+(*                       end in *)
+(*             T' ++ (f n1) *)
+(*         end *)
+(*     end in *)
+(*   f n. *)
   
-Definition gen_sub_tvar (E : env) (T2 : typ) : G typ :=
-  elems_ T2 (find_sub_tvar E T2). 
+(* Definition gen_sub_tvar (E : env) (T2 : typ) : G typ := *)
+(*   elems_ T2 (find_sub_tvar E T2).  *)
 
-Definition find_sup_tvar (E : env) (n1 : nat) : list typ :=
-  match get_bound E n1 with
-  | None => []
-  | Some T1 => 
-      let n := count_tvar E in
-      let fix f n2 :=
-        match n2 with
-        | O => []
-        | S n2 => 
-            match get_bound E n2 with
-            | None => []
-            | Some T2 => 
-                let T' := match sub_check' E T1 T2 with
-                          | true => [tvar n1]
-                          | _ => []
-                          end in
-                T' ++ (f n2)
-            end
-        end in
-      f n
-  end.
+(* (* This is actually incorrect! *) *)
+(* Definition find_sup_tvar (E : env) (n1 : nat) : list typ := *)
+(*   match get_bound E n1 with *)
+(*   | None => [] *)
+(*   | Some T1 =>  *)
+(*       let n := count_tvar E in *)
+(*       let fix f n2 := *)
+(*         match n2 with *)
+(*         | O => [] *)
+(*         | S n2 =>  *)
+(*             match get_bound E n2 with *)
+(*             | None => [] *)
+(*             | Some T2 =>  *)
+(*                 let T' := match sub_check' E T1 T2 with *)
+(*                           | true => [tvar n1] *)
+(*                           | _ => [] *)
+(*                           end in *)
+(*                 T' ++ (f n2) *)
+(*             end *)
+(*         end in *)
+(*       f n *)
+(*   end. *)
 
-Definition gen_sup_tvar (E : env) (n1 : nat) : G typ :=
-  elems_ (tvar n1) (find_sup_tvar E n1). 
+(* Definition gen_sup_tvar (E : env) (n1 : nat) : G typ := *)
+(*   elems_ (tvar n1) (find_sup_tvar E n1).  *)
 
-Fixpoint gen_sub_typ (n : nat) (E : env) (T : typ) : G typ :=
-  match n with
-  | O => ret T                  (** [sub] is reflexive *)
-  | S n =>
-      let g1 :=
-        match T with
-        | top =>
-            (** any <: [top] *)
-            T1 <- gen_exact_typ n E ;;
-            match T1 with
-            | Some T1 => ret T1
-            | None => ret top
-            end
-        | tvar n => ret (tvar n)
-        | arrow T1 T2 =>
-            (** [S1] :> [T1] -> 
-                [S2] <: [T2] ->
-                arrow [S1] [S2] <: arrow [T1] [T2] 
-             *)
-            S1 <- gen_sup_typ n E T1;;
-            S2 <- gen_sub_typ n E T2;;
-            ret (arrow S1 S2)
-        | all T1 T2 =>
-            S1 <- gen_sup_typ n E T1;;
-            S2 <- gen_sub_typ n (ebound E T1) T2;;
-            ret (all S1 S2)
-        end in
-      let g2 := map ret (find_sub_tvar E T) in
-      oneOf_ (ret T) ((ret T) :: g1 :: g2)
-  end
-with
-gen_sup_typ (n : nat) (E : env) (T : typ) : G typ :=
-  match n with
-  | O => ret T                  (** [sup] is reflexive *)
-  | S n =>
-      let g1 :=
-        match T with
-        | top => ret top        (** [top] is the top *)
-        | tvar n => gen_sup_tvar E n
-        | arrow T1 T2 =>
-            S1 <- gen_sub_typ n E T1;;
-            S2 <- gen_sup_typ n E T2;;
-            ret (arrow S1 S2)
-        | all T1 T2 =>
-            S1 <- gen_sub_typ n E T1;;
-            S2 <- gen_sup_typ n (ebound E T1) T2;;
-            ret (all S1 S2)
-        end in
-      oneOf [ret T ; g1]
-  end
-.
+(* Fixpoint gen_sub_typ (n : nat) (E : env) (T : typ) : G typ := *)
+(*   match n with *)
+(*   | O => ret T                  (** [sub] is reflexive *) *)
+(*   | S n => *)
+(*       let g1 := *)
+(*         match T with *)
+(*         | top => *)
+(*             T1 <- gen_exact_typ n E ;; *)
+(*             match T1 with *)
+(*             | Some T1 => ret T1 *)
+(*             | None => ret top *)
+(*             end *)
+(*         | tvar n => ret (tvar n) *)
+(*         | arrow T1 T2 => *)
+(*             S1 <- gen_sup_typ n E T1;; *)
+(*             S2 <- gen_sub_typ n E T2;; *)
+(*             ret (arrow S1 S2) *)
+(*         | all T1 T2 => *)
+(*             S1 <- gen_sup_typ n E T1;; *)
+(*             S2 <- gen_sub_typ n (ebound E T1) T2;; *)
+(*             ret (all S1 S2) *)
+(*         end in *)
+(*       let g2 := map ret (find_sub_tvar E T) in *)
+(*       oneOf_ (ret T) ((ret T) :: g1 :: g2) *)
+(*   end *)
+(* with *)
+(* gen_sup_typ (n : nat) (E : env) (T : typ) : G typ := *)
+(*   match n with *)
+(*   | O => ret T                  (** [sup] is reflexive *) *)
+(*   | S n => *)
+(*       let g1 := *)
+(*         match T with *)
+(*         | top => ret top        (** [top] is the top *) *)
+(*         | tvar n => gen_sup_tvar E n *)
+(*         | arrow T1 T2 => *)
+(*             S1 <- gen_sub_typ n E T1;; *)
+(*             S2 <- gen_sup_typ n E T2;; *)
+(*             ret (arrow S1 S2) *)
+(*         | all T1 T2 => *)
+(*             S1 <- gen_sub_typ n E T1;; *)
+(*             S2 <- gen_sup_typ n (ebound E T1) T2;; *)
+(*             ret (all S1 S2) *)
+(*         end in *)
+(*       oneOf [ret T ; g1] *)
+(*   end *)
+(* . *)
 
-Definition c_gen_sub_typ g n E : G (option typ) :=
-  oT <- (g n E) ;;
-  match oT with
-  | None => ret None 
-  | Some T => liftM Some (gen_sub_typ n E T)
-  end.
-
-Definition c_gen_sup_typ g n E : G (option typ) :=
-  oT <- (g n E) ;;
-  match oT with
-  | None => ret None 
-  | Some T => liftM Some (gen_sup_typ n E T)
-  end.
-
-      
-(** ** Generate System F <:
-    
-    - Generate a type to be used as the super type of the program
-    - Widen the type of an exact type step by step
-*)
-
-(** Generate a [typ] *)
-(** Reworked [gen_typ] : allow bare [top]s and [arrow]s *)
 Definition fetch_var_typs (E : env) : list typ :=
   let nvar := count_var E in
   let fix f n :=
@@ -301,228 +361,94 @@ Definition fetch_var_typs (E : env) : list typ :=
   f nvar.
 
 
+Definition find_sub_var_typs (E : env) (T : typ) : list typ :=
+  List.filter (fun T' => sub_check' E T' T) (fetch_var_typs E). 
 
-(** for each [var] in the env, "upcasts" can be done to it *)
-Definition fetch_good_typs (E : env) : list typ :=
-  let vars := fetch_var_typs E in
+Definition find_sup_var_typs (E : env) (T : typ) : list typ :=
+  List.filter (sub_check' E T) (fetch_var_typs E). 
+
+Definition find_sub_tvar_typs (E : env) (T : typ) : list typ :=
   let ntvars :=  count_tvar E in
   let fix f n :=
     match n with
     | O => []
-    | S n => (tvar n) :: f n
+    | S n => n :: f n
     end in
-  let tvars := f ntvars in 
-  List.fold_right
-    (fun v acc =>
-       acc ++ match v with
-              | tvar n =>
-                  v ::          (** bound var itself *)
-                    match get_bound E n with
-                    | Some T => (** upcasts to its super type *)
-                        List.filter (sub_check' E T) tvars
-                    | None => []
-                    end
-              (** More can be done here: analyze structure of the typ *)
-              | _ => [v]
-              end)
-    [] vars.
-    
-(** Motivation: 
+  map tvar
+      (List.filter
+         (fun n =>
+            match get_bound E n with
+            | Some T' => sub_check' E T' T
+            | _ => false
+            end)
+         (f ntvars)).
 
-    ∀ top. ∀ <0>. ∀ <0>. <0> -> ◻ *)
-Example env_with_sub :=
-  (evar
-     (ebound
-        (ebound
-           (ebound empty
-                   top)
-           (tvar 0))
-        (tvar 1))
-     (tvar 0)). 
 
-Eval cbv in fetch_var_typs env_with_sub. 
-Eval cbv in fetch_good_typs env_with_sub. 
-
-Definition gen_typ0 (E : env) (r : bool) : G typ := 
-  if r
-  then                          (** Restricted: must be sub bound [var] *)
-    freq [(1, ret top);
-          let Ts := fetch_good_typs E in
-          (List.length Ts, elems_ top Ts)]
-  else                          (** Any bound [var] or [tvar] suffice *)
-    freq [(1, ret top);
-          let n'' := count_tvar E in
-          (n'', n' <- choose(0, n'');; ret (tvar n'));
-          let vs := fetch_var_typs E in
-          (List.length vs, elems_ top vs)].
-
-Fixpoint gen_typ (n : nat) (E : env) (r : bool) {struct n} : G typ :=
+Fixpoint gen_sub_typ (n : nat) (E : env) (T : typ) {struct n} : G typ :=
   match n with
-  | O =>
-      gen_typ0 E r
+  | O => ret T                  (** [sub] is reflexive *)
   | S n =>
-      freq [(1, gen_typ0 E r) ;
-            (1, T1 <- gen_typ (n - 1) E false ;;
-                T2 <- gen_typ n (ebound E T1) r ;;
-                ret (all T1 T2)) ; 
-            (1, T1 <- gen_typ (n - 1) E false ;;
-                T2 <- gen_typ n (evar E T1) r ;;
-                ret (arrow T1 T2))]
-  end.
-
-Sample (gen_typ 4 empty true).
-
-Definition gen_opt_typ (n : nat) (E : env) (r : bool) : G (option typ) :=
-  fmap Some (gen_typ n E r).
-
-(** Generate a [term] *)
-
-(** Find a bound var that is of a subtype of [T]  *)
-Fixpoint get_bound_sub_vars (T : typ) (E : env) : list term :=
-  let n := count_var E in
-  let fix f n1 :=
-    match n1 with
-    | O => []
-    | S n1 => 
-        match get_var E n1 with
-        | None => []
-        | Some T1 => 
-            let T' := match sub_check' E T1 T with
-                      | true => [var n1]
-                      | _ => []
-                      end in
-            T' ++ (f n1)
-        end
-    end in
-  f n.
-
-Fixpoint get_bound_sup_vars (T : typ) (E : env) : list term :=
-  let n := count_var E in
-  let fix f n1 :=
-    match n1 with
-    | O => []
-    | S n1 => 
-        match get_var E n1 with
-        | None => []
-        | Some T1 => 
-            let T' := match sub_check' E T T1 with
-                      | true => [var n1]
-                      | _ => []
-                      end in
-            T' ++ (f n1)
-        end
-    end in
-  f n.
-
-Definition gen_bound_sub_vars T E : G (option term) :=
-  elems_ None (map Some (get_bound_sub_vars T E)).
-
-Definition gen_bound_sup_vars T E : G (option term) :=
-  elems_ None (map Some (get_bound_sup_vars T E)).
-
-
-Fixpoint gen_sub_term0 (E : env) (T : typ) : G (option term) :=
-  let g : (G (option term)) :=
-    match T with
-    | arrow T1 T2 =>
-        liftM (abs T1) (gen_sub_term0 (evar E T1) T2)
-    | all T1 T2 =>
-        liftM (tabs T1)
-              (gen_sub_term0 (ebound E T1) T2)
-    | _ => ret None
-    end
-  in     
-  backtrack [(1, g); (1, (gen_bound_sub_vars T E))].
-
-Fixpoint gen_sup_term0 (E : env) (T : typ) : G (option term) :=
-  let g : (G (option term)) :=
-    match T with
-    | arrow T1 T2 =>
-        liftM (abs T1) (gen_sup_term0 (evar E T1) T2)
-    | all T1 T2 =>
-        liftM (tabs T1)
-              (gen_sup_term0 (ebound E T1) T2)
-    | _ => ret None
-    end
-  in     
-  backtrack [(1, g); (1, (gen_bound_sup_vars T E))].
-
-
-(** generate operands to functions in the context *)
-Definition michalsub (E : env) (T : typ) : list typ :=
-  let n := count_var E in
-  let fix f2 T' :=
-    match T' with
-    | arrow T1 T2 =>
-        (** don't need to shift type here: no intro of tvar *)
-        match sub_check' E T2 T with
-        | true => [T1]
-        | _ => []
-        end ++ f2 T2
-    | _ => []
-    end in
-  let fix f n1 :=
-    match n1 with
-    | O => []
-    | S n1 => 
-        match get_var E n1 with
-        | Some T' => f2 T'
-        | None => []
-        end ++ f n1
-    end in
-  f n.
-
-(** not useful? *)
-Definition c_michalsub (g : G (option typ)) (E : env) (T : typ)
-  : G (option typ) :=
-  oneOf_ g (g :: (map (fun x => ret (Some x)) (michalsub E T))).
-
-
-(** Generate a term of a subtype of [T] *)
-Fixpoint gen_sub_term (n : nat) (E : env) (T : typ) : G (option term) :=
-  match n with
-  | O => gen_sub_term0 E T
-  | S n =>
-      let n' := n - 2 in (* n - n / 2 in *)
-      (** Base Case *)
-      let g0 := gen_sub_term0 E T in
-      (** Generate by typ *)
-      let g1 := 
+      let g1 :=
         match T with
-        | arrow T1 T2 =>
-            T1' <- (c_gen_sup_typ (fun _ _ => ret T1) n E) ;;
-            t2 <- (gen_sub_term n (evar E T1') T2) ;;
-            ret (abs T1' t2)
+        | top =>                
+            oT <- gen_exact_typ n E;;
+            ret (match oT with None => top | Some t => t end)
+        | tvar n => ret (tvar n)
+        | arrow T1 T2 => 
+            S1 <- gen_sup_typ n E T1;;
+            S2 <- gen_sub_typ n E T2;;
+            ret (arrow S1 S2)
         | all T1 T2 =>
-            T1' <- (c_gen_sup_typ (fun _ _ => ret T1) n E) ;;
-            t2 <- (gen_sub_term n (ebound E T1') T2) ;;
-            ret (tabs T1' t2)
-        | _ => g0
+            S1 <- gen_sup_typ n E T1;;
+            S2 <- gen_sub_typ n (ebound E T1) T2;;
+            ret (all S1 S2)
         end in
-      (** Generate App *)
       let g2 :=
-        (** restricted: to generate the operand term *)
-        T1 <- c_michalsub (gen_opt_typ n' E true) E T;;
-        (** generate [t1] of a subtype of [T1 -> T] *)
-        t1 <- gen_sub_term n' E (arrow T1 T);;
-        (** generate [t2] of a subtype of [T1] *)
-        t2 <- gen_sub_term n' E T1;;
-        returnGen (Some (app t1 t2))
-      in
-      (** Generate TApp : [t1'] is [(tabs T1 t1) T2] <: [T] *)
-      let g3 :=
-        (** unrestricted: typ can be any *)
-        T1 <- gen_opt_typ n' E false;; 
-        T2 <- c_gen_sub_typ (fun _ _ => ret T1) n' E;;
-        t1' <- gen_sub_term n' E (all T1 (tshift 0 T)) ;;
-        returnGen (Some (tapp t1' T2))
-      in backtrack [(1, g0); (1, g1); (1, g2); (1, g3)]
+        elems_ T ((find_sub_var_typs E T) ++ (find_sub_tvar_typs E T)) in
+      let g2' := T <- g2 ;; gen_sub_typ n E T in
+      oneOf [ret T; g1; g2; g2']
+  end
+with
+gen_sup_typ (n : nat) (E : env) (T : typ) {struct n} : G typ :=
+  match n with
+  | O => ret T                  (** [sup] is reflexive *)
+  | S n =>
+      let g1 :=
+        match T with
+        | top => ret top        (** [top] is the top *)
+        | tvar n' =>
+            match get_bound E n' with
+            | Some T => gen_sup_typ n E T
+            | _ => ret (tvar n')
+            end
+        | arrow T1 T2 =>
+            S1 <- gen_sub_typ n E T1;;
+            S2 <- gen_sup_typ n E T2;;
+            ret (arrow S1 S2)
+        | all T1 T2 =>
+            S1 <- gen_sub_typ n E T1;;
+            S2 <- gen_sup_typ n (ebound E T1) T2;;
+            ret (all S1 S2)
+        end in
+      let g2 := elems_ top (find_sup_var_typs E T) in
+      let g2' := T <- g2 ;; gen_sup_typ n E T in 
+      oneOf [ret T; g1; g2; g2']
   end
 .
 
-Sample (gen_opt_typ 2 empty true).
+Definition c_gen_sub_typ g n E : G (option typ) :=
+  oT <- (g n E) ;;
+  match oT with
+  | None => ret None
+  | Some T => liftM Some (gen_sub_typ n E T)
+  end.
 
-Sample (gen_sub_term 3 empty top).
+Definition c_gen_sup_typ g n E : G (option typ) :=
+  oT <- (g n E) ;;
+  match oT with
+  | None => ret None
+  | Some T => liftM Some (gen_sup_typ n E T)
+  end.
 
 Definition max_dec n m : nat :=
   if le_gt_dec n m then m else n.
@@ -534,4 +460,3 @@ Fixpoint measure_max_typ (T : typ) : nat :=
   | arrow T1 T2 => 1 + max_dec (measure_max_typ T1) (measure_max_typ T2)
   | all T1 T2 => 1 + max_dec (measure_max_typ T1) (measure_max_typ T2)
   end.
-
