theories/GeneratorExample.v
@@ -1,0 +1,27 @@
+From FSUB Require Import
+     QCLibs
+     FSub
+     Decidable
+     GeneratorSub.
+
+(** Motivation [fetch_good_typs] : 
+    ∀ top. ∀ <0>. ∀ <0>. <0> -> ◻ *)
+Example env_with_sub :=
+  (evar
+     (ebound
+        (ebound
+           (ebound empty
+                   top)
+           (tvar 0))
+        (tvar 1))
+     (tvar 0)). 
+
+Eval cbv in fetch_var_typs env_with_sub. 
+Eval cbv in fetch_good_typs env_with_sub. 
+
+
+Example repl_ty :=
+  (arrow (tvar 0) (arrow (tvar 1) (all top (arrow (tvar 1) (tvar 0))))).
+
+Sample (gen_replace repl_ty).
+
