theories/Mutant.v
@@ -16,7 +16,7 @@ Definition prop_gen_progress_nf (m : Mutant) :=
   let step' := pstep' in
   forAllMaybe (gen_exact_typ fuel_type empty) (fun T =>
   forAllMaybe (gen_exact_term fuel_type empty T) (fun t =>
-  forAll (gen_sup_typ fuel_type empty T) (fun T =>
+  forAll (gen_sup_typ fuel_type empty T) (fun _ =>
   whenFail ("Generated" ++ nl ++
             "[T]: " ++ show T ++ nl ++ 
             "[t]: " ++ show t ++ nl ++
@@ -34,29 +34,35 @@ Definition prop_gen_progress_nf (m : Mutant) :=
                | _ => false
                end))%bool))).
 
-(* QuickChick (prop_gen_progress_nf NoMutant). (* Correct ! *) *)
+QuickChick (prop_gen_progress_nf NoMutant). (* Correct ! *)
 
-(** Okay for WHNF *)
-(* QuickChick (prop_gen_progress_nf TShiftTVarAll).       (* 4 *) *)
-(* QuickChick (prop_gen_progress_nf TSubstTVarFlip).      (* 4 *) *)
-(* QuickChick (prop_gen_progress_nf TSubstTVarOverShift). (* 4 *) *)
-(* QuickChick (prop_gen_progress_nf SubstVarFlip).        (* 4 *) *)
-(* QuickChick (prop_gen_progress_nf SubstAbsNoIncr).      (* 4 *) *)
-(* QuickChick (prop_gen_progress_nf ShiftVarAll).         (* 4 *) *)
-(* QuickChick (prop_gen_progress_nf ShiftAbsNoIncr).      (* 4 *) *)
-(* QuickChick (prop_gen_progress_nf ShiftTypTAbsNoIncr).  (* 4 *) *)
-(* QuickChick (prop_gen_progress_nf TShiftAllNoIncr).     (* 4 *) *)
+(* (** Okay for WHNF *) *)
+QuickChick (prop_gen_progress_nf TShiftTVarAll).       (* 4 *)
+QuickChick (prop_gen_progress_nf TSubstTVarFlip).      (* 4 *)
+QuickChick (prop_gen_progress_nf TSubstTVarOverShift). (* 4 *)
+QuickChick (prop_gen_progress_nf SubstVarFlip).        (* 4 *)
+QuickChick (prop_gen_progress_nf SubstAbsNoIncr).      (* 4 *)
+QuickChick (prop_gen_progress_nf ShiftVarAll).         (* 4 *)
+QuickChick (prop_gen_progress_nf ShiftAbsNoIncr).      (* 4 *)
+QuickChick (prop_gen_progress_nf ShiftTypTAbsNoIncr).  (* 4 *)
+QuickChick (prop_gen_progress_nf TShiftAllNoIncr).     (* 4 *)
 
-(** Okay for NF *)
-(* QuickChick (prop_gen_progress_nf TShiftTVarNoIncr).  (* 4 *) *)
-(* QuickChick (prop_gen_progress_nf SubstTAbsNoShift).  (* 4 *) *)
-(* QuickChick (prop_gen_progress_nf TSubstTVarNoShift). (* 4 *) *)
-(* QuickChick (prop_gen_progress_nf SubstVarNoDecr).    (* 4 *) *)
-(* QuickChick (prop_gen_progress_nf SubstAbsNoShift).   (* 4 *) *)
-(* QuickChick (prop_gen_progress_nf ShiftVarNoIncr).    (* 4 *) *)
+(* (** Okay for NF *) *)
+QuickChick (prop_gen_progress_nf TShiftTVarNoIncr).  (* 4 *)
+QuickChick (prop_gen_progress_nf SubstTAbsNoShift).  (* 4 *)
+QuickChick (prop_gen_progress_nf TSubstTVarNoShift). (* 4 *)
+QuickChick (prop_gen_progress_nf SubstVarNoDecr).    (* 4 *)
+QuickChick (prop_gen_progress_nf SubstAbsNoShift).   (* 4 *)
+QuickChick (prop_gen_progress_nf ShiftVarNoIncr).    (* 4 *)
 
 (** Nope!  *)
-(* QuickChick (prop_gen_progress_nf TSubstAllNoTShift). (* Nope *) *)
+(** Hard to generate : 
+    - can be spotted only in NF
+    - generate RHS in [tapp] that uses [typ]s from the [env]
+    - RHS needs to be used in LHS
+ *)
+QuickChick (prop_gen_progress_nf TSubstAllNoTShift). (* Nope *)
+
 
 
 (** ** [C7] Weak Progress *)
@@ -83,25 +89,25 @@ Definition prop_gen_progress (m : Mutant) :=
                | _ => false
                end))%bool))).
 
-(* QuickChick (prop_gen_progress NoMutant). (* Correct ! *) *)
+QuickChick (prop_gen_progress NoMutant). (* Correct ! *)
 
 (** Should be detectable *)
-(* QuickChick (prop_gen_progress TShiftTVarAll).       (* 4 *) *)
-(* QuickChick (prop_gen_progress TSubstTVarFlip).      (* 4 *) *)
-(* QuickChick (prop_gen_progress TSubstTVarOverShift). (* 4 *) *)
-(* QuickChick (prop_gen_progress SubstVarFlip).        (* 4 *) *)
-(* QuickChick (prop_gen_progress SubstAbsNoIncr).      (* 4 *) *)
-(* QuickChick (prop_gen_progress ShiftVarAll).         (* 4 *) *)
-(* QuickChick (prop_gen_progress ShiftAbsNoIncr).      (* 4 *) *)
-(* QuickChick (prop_gen_progress ShiftTypTAbsNoIncr).  (* 4 *) *)
-(* QuickChick (prop_gen_progress TShiftAllNoIncr).     (* 4 *) *)
+QuickChick (prop_gen_progress TShiftTVarAll).       (* 4 *)
+QuickChick (prop_gen_progress TSubstTVarFlip).      (* 4 *)
+QuickChick (prop_gen_progress TSubstTVarOverShift). (* 4 *)
+QuickChick (prop_gen_progress SubstVarFlip).        (* 4 *)
+QuickChick (prop_gen_progress SubstAbsNoIncr).      (* 4 *)
+QuickChick (prop_gen_progress ShiftVarAll).         (* 4 *)
+QuickChick (prop_gen_progress ShiftAbsNoIncr).      (* 4 *)
+QuickChick (prop_gen_progress ShiftTypTAbsNoIncr).  (* 4 *)
+QuickChick (prop_gen_progress TShiftAllNoIncr).     (* 4 *)
 
 (** Should only work under NF *)
-(* QuickChick (prop_gen_progress TShiftTVarNoIncr).  (* Nope *) *)
-(* QuickChick (prop_gen_progress SubstTAbsNoShift).  (* Nope *) *)
-(* QuickChick (prop_gen_progress TSubstTVarNoShift). (* Nope *) *)
-(* QuickChick (prop_gen_progress SubstVarNoDecr).    (* Nope *) *)
-(* QuickChick (prop_gen_progress TSubstAllNoTShift). (* Nope *) *)
-(* QuickChick (prop_gen_progress SubstAbsNoShift).   (* Nope *) *)
-(* QuickChick (prop_gen_progress ShiftVarNoIncr).    (* Nope *) *)
-(* QuickChick (prop_gen_progress ShiftVarNoIncr).    (* Nope *) *)
+QuickChick (prop_gen_progress TShiftTVarNoIncr).  (* Nope *)
+QuickChick (prop_gen_progress SubstTAbsNoShift).  (* Nope *)
+QuickChick (prop_gen_progress TSubstTVarNoShift). (* Nope *)
+QuickChick (prop_gen_progress SubstVarNoDecr).    (* Nope *)
+QuickChick (prop_gen_progress TSubstAllNoTShift). (* Nope *)
+QuickChick (prop_gen_progress SubstAbsNoShift).   (* Nope *)
+QuickChick (prop_gen_progress ShiftVarNoIncr).    (* Nope *)
+QuickChick (prop_gen_progress ShiftVarNoIncr).    (* Nope *)
