theories/MutantExample.v
@@ -1,0 +1,40 @@
+From FSUB Require Import
+     QCLibs
+     FSub
+     Decidable
+     MutantInterface.
+
+(** * MutantExample: Debug Mutants *)
+(** ** TSubstAllNoTShift *)
+Module TSubstAllNoTShift. 
+  Example tm1 :=
+    tabs top
+         (tabs top
+               (tapp (tabs top
+                           (tabs top
+                                 (abs (all (tvar 0)
+                                           (arrow (arrow (tvar 0) (tvar 1))
+                                                  (arrow (tvar 2) (tvar 3))))
+                                      (var 0))))
+                     (arrow (tvar 0) (tvar 1)))).
+  Eval cbv in get_typ' empty tm1.
+
+  (* Already in value form *)
+  Eval cbn in step'' (TSubstAllNoTShift) tm1.
+
+  (* But not in normal form *)
+  Example otm2 :=
+    pstep' (NoMutant) tm1.
+
+  Example otm2' :=
+    pstep' (TSubstAllNoTShift) tm1.
+
+  Example TSubstAllNoTShift_tm_diff :
+    otm2 <> otm2'.
+  Proof. cbn. easy. Qed.
+
+
+  Example TSubstAllNoTShift_diff' :
+    (tm2 <- otm2;; get_typ' empty tm2) <> (tm2' <- otm2';; get_typ' empty tm2').
+  Proof. cbn. easy. Qed.
+End TSubstAllNoTShift.
