theories/Reduction.v
@@ -2,7 +2,51 @@ From FSUB Require Import
      QCLibs
      FSub
      Decidable.
-(** * Reduction: Semantics *)
+(** * Reduction : Executable Semantics *)
+(** ** Reduction Semantics
+
+    The equivalence of original reduction semantics in POPLMark Challenge
+
+ *)
+Fixpoint ctx_inj (t : term) : option (ctx * term).
+  refine
+    (match t with
+     | app t1 t2 => _
+     | tapp t1 T2 =>
+         if dc_value t1 then ret (c_hole, t)
+         else '(c1, t1) <- ctx_inj t1;; ret (c_typefun c1 T2, t1)
+     | _ => ret (c_hole, t)
+     end).
+  destruct (reflect_value t1).
+  - (* [t1] is a value, inject context on [t2] *)
+    refine ('(c2, t2) <- ctx_inj t2;; ret (c_apparg v c2, t2)).
+  - (* [t1] is not a value, inject context on [t1] *)
+    refine ('(c1, t1) <- ctx_inj t1;; ret (c_appfun c1 t2, t1)).
+Defined.
+
+Fixpoint step (n : nat) (t : term) {struct n} : result :=
+  let step_ctx n t :=
+    match ctx_inj t with
+    | None => Result None
+    | Some (c', t') => 
+        match step n t' with
+        | Result (Some t'') => Result (Some (ctx_app c' t''))
+        | rst => rst
+        end
+    end in
+  match n with
+  | O => OutOfFuel
+  | S n =>            
+      match t with
+      | app (abs _ t12) t2 =>
+          if dc_value t2 then Result (Some (subst t12 0 t2))
+          else step_ctx n t
+      | tapp (tabs T11 t12) T2 => Result (Some (subst_typ t12 0 T2))
+      | _ => step_ctx n t
+      end
+  end.
+
+(** Unverified yet *)
 
 (** ** Alternative Semantics
     
@@ -79,3 +123,4 @@ Theorem step'_correct :
 Proof.
   intros. split; [apply step'_implies_red' | apply red'_implies_step'].
 Qed. 
+
